move proofs of correcness of Inv to Mid as it is on Z not on lists, translate proofs to list, define Inv25519 over lists.

Low/Inv25519.v
@@ -3,14 +3,19 @@ Require Import Tweetnacl.ListsOp.Export.
 Require Import Tweetnacl.Low.Inv25519_gen.
 Require Import Tweetnacl.Low.M.
 Require Import Tweetnacl.Low.S.
+Require Import Tweetnacl.Mid.Inv25519.
 
 Open Scope Z.
 
+(*
+ * Define the iteration step over Lists
+ *)
 Definition step_pow := step_pow M Sq.
 
-Definition step_pow_Z a c g := let c0 := c*c in if Zneq_bool a 1 && Zneq_bool a 3 then c0*g else c0.
-
-Lemma step_pow_Z_GF_eq: forall a c g,
+(*
+ * Equivalence over GF.
+ *)
+Local Lemma step_pow_Z_GF_eq: forall a c g,
   Zlength c = 16 ->
   Zlength g = 16 ->
   ZofList 16 (step_pow a c g) :𝓖𝓕  = (step_pow_Z a (ZofList 16 c) (ZofList 16 g)) :𝓖𝓕 .
@@ -23,19 +28,9 @@ rewrite Zmult_mod mult_GF_Zlengh -?Zmult_mod => //.
 apply M_Zlength => //.
 Qed.
 
-Function pow_fn_rev_Z (a b:Z) (c g: Z) {measure Z.to_nat a} : (Z) :=
-  if (a <=? 0)
-    then c
-    else
-      let prev := pow_fn_rev_Z (a - 1) b c g in 
-        step_pow_Z (b - 1 - a) prev g.
-Proof. intros. apply Z2Nat.inj_lt ; move: teq ; rewrite Z.leb_gt => teq; omega. Defined.
-
-Lemma pow_fn_rev_Z_n : forall a b c g,
-  0 < a ->
-  pow_fn_rev_Z a b c g = step_pow_Z (b - 1 - a) (pow_fn_rev_Z (a - 1) b c g) g.
-Proof. intros. rewrite pow_fn_rev_Z_equation. flatten; apply Zle_bool_imp_le in Eq; omega. Qed.
-
+(*
+ * Define the recursion over list
+ *)
 Definition pow_fn_rev := pow_fn_rev M Sq.
 
 Lemma pow_fn_rev_0 : forall b c g,
@@ -125,338 +120,30 @@ Proof.
   apply Sq_bound_Zlength.
 Qed.
 
-(*****************************************************************************************
- *   DEFINE SEMANTIC
- *)
+(* Define Inv25519 *)
 
+Definition Inv25519 (x:list Z) : (list Z) := pow_fn_rev 254 254 x x.
 
-Inductive expr_inv :=
-  | R_inv : expr_inv
-  | M_inv : expr_inv -> expr_inv -> expr_inv
-  | S_inv : expr_inv -> expr_inv
-  | P_inv : expr_inv -> positive -> expr_inv.
+Lemma Inv25519_bound_Zlength : forall g,
+  Zlength g = 16 ->
+  Forall (fun x => -38 <= x < Z.pow 2 16 + 38) g ->
+  Forall (fun x => -38 <= x < Z.pow 2 16 + 38) (Inv25519 g).
+Proof. intros; rewrite /Inv25519; apply pow_fn_rev_bound_Zlength => //. Qed.
 
-Inductive formula_inv := 
-  | Eq_inv : expr_inv -> expr_inv -> formula_inv.
+Lemma Inv25519_Zlength : forall g,
+  Zlength g = 16 -> 
+  Zlength (Inv25519 g) = 16.
+Proof. intros; rewrite /Inv25519; apply pow_fn_rev_Zlength => //. Qed.
 
-Fixpoint expr_inv_denote v env (m : expr_inv) : Z :=
-  match m with
-  | R_inv     => term_denote env v
-  | M_inv x y => (expr_inv_denote v env x) * (expr_inv_denote v env y)
-  | S_inv x => (expr_inv_denote v env x) * (expr_inv_denote v env x)
-  | P_inv x p => Z.pow (expr_inv_denote v env x) (Z.pos p)
-  end.
+Lemma Inv25519_Z_GF : forall g,
+  Zlength g = 16 ->
+  ZofList 16 (Inv25519 g) :𝓖𝓕  = (Inv25519_Z (ZofList 16 g)) :𝓖𝓕 .
+Proof. intros; rewrite /Inv25519 /Inv25519_Z; apply pow_fn_rev_Z_GF => //. Qed.
 
-Definition formula_inv_denote v env (t : formula_inv) : Prop :=
-  match t with
-  | Eq_inv x y     => expr_inv_denote v env x = expr_inv_denote v env y
-  end.
-
-(*****************************************************************************************
- *   DECIDE EQUALITY
- *)
-
-Fixpoint compute_pow_expr_inv (t : expr_inv) : Z := match t with
-  | R_inv   => 1
-  | M_inv x y => (compute_pow_expr_inv x) + (compute_pow_expr_inv y)
-  | S_inv x => 2 * (compute_pow_expr_inv x)
-  | P_inv x p => (Z.pos p) * (compute_pow_expr_inv x)
-  end.
-
-Lemma compute_pow_expr_inv_pos : forall l, 0 <= compute_pow_expr_inv l.
-Proof. induction l ; go. Qed.
-
-Lemma compute_pow_expr_M_inv_pos : forall l l', 0 <= compute_pow_expr_inv (M_inv l l').
-Proof. intros ; simpl.
-assert(H := compute_pow_expr_inv_pos l).
-assert(H' := compute_pow_expr_inv_pos l') ; omega.
-Qed.
-
-Lemma compute_pow_expr_S_inv_pos : forall l, 0 <= compute_pow_expr_inv (S_inv l).
-Proof. intros ; simpl.
-assert(H := compute_pow_expr_inv_pos l) ; omega.
-Qed.
-
-Lemma compute_pow_expr_inv_denote: forall env v l,
-  expr_inv_denote v env l = Z.pow (term_denote env v) (compute_pow_expr_inv l).
-Proof.
-  induction l.
-  simpl ; ring.
-  assert(Hl1:= compute_pow_expr_inv_pos l1).
-  assert(Hl2:= compute_pow_expr_inv_pos l2).
-  simpl; rewrite IHl1 IHl2 -Z.pow_add_r; go.
-  assert(Hl1:= compute_pow_expr_inv_pos l).
-  simpl; rewrite IHl -Z.pow_add_r ; go.
-  f_equal ; omega.
-  assert(Hl1:= compute_pow_expr_inv_pos l).
-  assert(Hp:= Pos2Z.is_nonneg p).
-  simpl; rewrite IHl -Z.pow_mul_r; go.
-  by rewrite Z.mul_comm.
-Qed.
-
-Fixpoint decide_expr_inv_eq (l1 l2:expr_inv) :=
-  Z.eqb (compute_pow_expr_inv l1) (compute_pow_expr_inv l2).
-
-Lemma decide_expr_inv_eq_refl_impl : forall l1 l2, 
-  Z.eqb (compute_pow_expr_inv l1) (compute_pow_expr_inv l2) = true ->
-  (compute_pow_expr_inv l1) = (compute_pow_expr_inv l2).
-Proof. move=> l1 l2; rewrite Z.eqb_eq //. Qed.
-
-Lemma decide_expr_inv_eq_impl:
-  forall v env l l', 
-  decide_expr_inv_eq l l' = true ->
-  expr_inv_denote v env l = expr_inv_denote v env l'.
-Proof.
-intros; rewrite ?compute_pow_expr_inv_denote; f_equal.
-gen l'; induction l ; destruct l' ; auto => H;
-apply decide_expr_inv_eq_refl_impl in H ; by rewrite H.
-Qed.
-
-Definition decide_formula_inv (f : formula_inv) : bool := match f with
-  | Eq_inv x y => decide_expr_inv_eq x y
-  end.
-
-Lemma decide_formula_inv_impl : forall v env f, decide_formula_inv f = true -> formula_inv_denote v env f.
-Proof. move=> v env [? ?]. by apply decide_expr_inv_eq_impl. Qed.
-
-(* Weaponize our expression so we can translate functions *)
-
-
-Definition step_inv a c g : expr_inv := 
-  let c0 := (S_inv c) in if negb (Nat.eqb a 1) && negb (Nat.eqb a 3) then M_inv c0 g else c0.
-
-Lemma step_inv_step_pow_eq : forall v env a c g,
-  expr_inv_denote v env (step_inv (Z.to_nat a) c g) =  step_pow_Z a (expr_inv_denote v env c) (expr_inv_denote v env g).
-Proof.
-  intros.
-  rewrite /step_inv /step_pow_Z.
-  flatten.
-  reflexivity.
-  exfalso.
-  Focus 1.
-  apply andb_true_iff in Eq.
-  destruct Eq as [Eq2 Eq4].
-  apply andb_false_iff in Eq0.
-  apply negb_true_iff in Eq2.
-  apply negb_true_iff in Eq4.
-  apply beq_nat_false in Eq2.
-  apply beq_nat_false in Eq4.
-  destruct Eq0 as [Eq|Eq].
-  rewrite /Zneq_bool in Eq ; flatten Eq.
-  apply Z.compare_eq_iff in Eq0.
-  go.
-  rewrite /Zneq_bool in Eq ; flatten Eq.
-  apply Z.compare_eq_iff in Eq0.
-  go.
-  exfalso.
-  Focus 1.
-  apply andb_true_iff in Eq0.
-  destruct Eq0 as [Eq2 Eq4].
-  assert(a < 0 \/ 0 <= a) by omega.
-  destruct H.
-  assert(Z.to_nat a = 0%nat).
-  Search Z.to_nat Z.lt.
-  unfold Z.to_nat.
-  destruct a => //.
-  rewrite H0 in Eq.
-  by compute in Eq.
-  apply andb_false_iff in Eq.
-  destruct Eq as [Eq|Eq];
-  apply negb_false_iff in Eq ; apply beq_nat_true in Eq;
-  apply (f_equal Z.of_nat) in Eq;
-  rewrite Z2Nat.id in Eq; try assumption;
-  compute in Eq;
-  subst a;
-  by compute in Eq2,Eq4.
-  reflexivity.
-Qed.
-
-Close Scope Z.
-
-Fixpoint pow_inv (a b : nat) (c g: expr_inv) : expr_inv := match a with
-  | 0 => c
-  | S n => let prev := pow_inv n b c g in 
-              step_inv (b - 1 - a) prev g
-  end.
-
-Open Scope Z.
-
-Lemma pow_inv_pow_fn_rev_eq : forall v env a b c g,
-  expr_inv_denote v env (pow_inv (Z.to_nat a) (Z.to_nat b) c g) =  pow_fn_rev_Z a b (expr_inv_denote v env c) (expr_inv_denote v env g).
-Proof.
-  intros.
-  destruct a; intros.
-  go.
-  2: go.
-  remember (Z.pos p) as a.
-  assert(0 <= a).
-    subst; apply Zle_0_pos.
-  clears p.
-  gen b c g.
-  gen a.
-  apply (natlike_ind (fun a => forall (b : ℤ) (c g : expr_inv),
-expr_inv_denote v env (pow_inv (Z.to_nat a) (Z.to_nat b) c g) =
-pow_fn_rev_Z a b (expr_inv_denote v env c) (expr_inv_denote v env g))).
-  go.
-  intros a Ha IHa b c g.
-  orewrite pow_fn_rev_Z_n.
-  oreplace (Z.succ a - 1) a.
-  replace ((Z.to_nat (Z.succ a))) with (S (Z.to_nat a)).
-  2: rewrite Z2Nat.inj_succ //.
-  simpl.
-  replace (Z.to_nat b - 1 - S (Z.to_nat a))%nat with (Z.to_nat (b - 1 - Z.succ a)).
-  rewrite step_inv_step_pow_eq IHa //.
-  orewrite Z2Nat.inj_sub.
-  replace ((Z.to_nat (Z.succ a))) with (S (Z.to_nat a)).
-  2: rewrite Z2Nat.inj_succ //.
-  f_equal.
-  orewrite Z2Nat.inj_sub.
-  reflexivity.
-Qed.
-
-Close Scope Z.
-
-(* (**************************************************************************
- * Environment management tactics
- *)
-Require Export Coq.Lists.List.
-
-Ltac inList x xs :=
-  match xs with
-  | tt => false
-  | (x, _) => true
-  | (_, ?xs') => inList x xs'
-  end.
-
-Ltac addToList x xs :=
-  idtac "add_in" x xs;
-  let b := inList x xs in
-  match b with
-  | true => idtac "yes" ; xs
-  | false => idtac "nope" ; constr:((x, xs))
-  end.
-
-Ltac lookup x xs :=
-  match xs with
-  | (x, _) => constr:(1%positive)
-  | (_, ?xs') =>
-    let n := lookup x xs' in
-    constr:(Pos.succ n)
-  end.
-
-Ltac allVar xs e :=
-  match e with
-  | Z0 => xs
-  | Zpos _ => xs
-  | Zneg _ => xs
-  | _ => idtac "add" ; addToList e xs
-  end.
-
-Ltac allVars xs e ::=
-  match e with
-  | ?P = ?Q =>
-    let xs := allVars xs P in
-    allVars xs Q
-  | pow_fn_rev_Z _ _ ?X ?Y =>
-    idtac X;
-    let xs := allVars xs X in
-    allVars xs Y
-  | Z.pow ?X ?Y => allVar xs X
-  | ?X => idtac X ; allVar xs X
-  | _ => xs
-  end. *)
-
-(**************************************************************************
- * Reflection tactics
- *)
-
-Ltac reifyValue env t :=
-  match t with
-  | ?X =>
-    let v := lookup X env in
-    constr:(R_inv)
-  | _ => constr:(R_inv)
-  end.
-
-Ltac reifyExpr env t :=
-  lazymatch t with
-  | pow_fn_rev_Z ?a ?b ?X ?Y =>
-    let x := reifyValue env X in
-    let y := reifyValue env Y in
-    constr:(pow_inv (Z.to_nat a) (Z.to_nat b) x y)
-  | ?X * ?Y =>
-    let x := reifyValue env X in
-    let y := reifyValue env Y in
-    constr:(M_inv x y)
-  | Z.pow ?X ?Y =>
-    let x := reifyValue env X in
-    match Y with
-      | Z.pos ?p => constr:(P_inv x p)
-      | _ => constr:(P_inv x 1%positive)
-    end
-  | ?X =>
-    let x := reifyValue env X in
-    constr:(R_inv)
-  end.
-
-Ltac reifyTerm env t :=
-  lazymatch t with
-   | ?X = ?Y =>
-      let x := reifyExpr env X in
-      let y := reifyExpr env Y in
-      constr:(Eq_inv x y)
-  end.
-
-Ltac functionalize xs :=
-  let rec loop n xs' :=
-    lazymatch xs' with
-    | tt => constr:(fun _ : positive => 0%Z)
-    | (?x, tt) => constr:(fun _ : positive => x)
-    | (?x, ?xs'') =>
-      let f := loop (Pos.succ n) xs'' in
-      constr:(fun m : positive => if (m =? n)%positive then x else f m)
-    end in
-  loop (1%positive) xs.
-
-(**************************************************************************
- * User interface tactics
- *)
-
-Open Scope Z.
-(* 
-Eval compute in Z.pow 2 255 - 21.
-Z.pow 2 255 - 21 = 57896044618658097711785492504343953926634992332820282019728792003956564819947
-*)
-
-Theorem Inversion_correct : forall x, pow_fn_rev_Z 254 254 x x = Z.pow x 57896044618658097711785492504343953926634992332820282019728792003956564819947.
-Proof.
-intros.
-  match goal with
-  | [ |- ?X ] =>
-    let xs := constr:((x, tt)) in
-    let env := functionalize xs in
-    let r1  := reifyTerm xs X in
-    pose xs;
-    pose env;
-    pose r1
-    end.
-    (* in theory we would use change, but here we need to proceed slightly differently *)
-    assert (
-      formula_inv_denote (Var 1) {| vars := z |} f ->
-      pow_fn_rev_Z 254 254 x x =
-      x ^ 57896044618658097711785492504343953926634992332820282019728792003956564819947).
-    {
-    subst f z.
-    rewrite /formula_inv_denote pow_inv_pow_fn_rev_eq.
-    go.
-    }
-    apply H ; clear H.
-    apply decide_formula_inv_impl.
-    (* at this point we don't need any hypothesis, this is purely computatinal *)
-    subst f.
-    clears.
-    compute.
-    reflexivity.
-Qed.
+Lemma Inv25519_Zpow_GF : forall g,
+  Zlength g = 16 ->
+  ZofList 16 (Inv25519 g) :𝓖𝓕  = (Z.pow (ZofList 16 g) (Z.pow 2 255 - 21)) :𝓖𝓕 .
+Proof. intros. rewrite Inv25519_Z_GF //.
+f_equal. apply Inv25519_Z_correct. Qed.
 
 Close Scope Z.
