Mid/Inv25519.v
@@ -1,0 +1,298 @@
+Require Import Tweetnacl.Libs.Export.
+Require Import Tweetnacl.ListsOp.Export.
+Require Import Tweetnacl.Low.M.
+Require Import Tweetnacl.Low.S.
+Open Scope Z.
+
+Definition step_pow_Z a c g := let c0 := c*c in if Zneq_bool a 1 && Zneq_bool a 3 then c0*g else c0.
+
+Function pow_fn_rev_Z (a b:Z) (c g: Z) {measure Z.to_nat a} : (Z) :=
+  if (a <=? 0)
+    then c
+    else
+      let prev := pow_fn_rev_Z (a - 1) b c g in 
+        step_pow_Z (b - 1 - a) prev g.
+Proof. intros. apply Z2Nat.inj_lt ; move: teq ; rewrite Z.leb_gt => teq; omega. Defined.
+
+Lemma pow_fn_rev_Z_n : forall a b c g,
+  0 < a ->
+  pow_fn_rev_Z a b c g = step_pow_Z (b - 1 - a) (pow_fn_rev_Z (a - 1) b c g) g.
+Proof. intros. rewrite pow_fn_rev_Z_equation. flatten; apply Zle_bool_imp_le in Eq; omega. Qed.
+
+Definition Inv25519_Z (x:Z) : Z := pow_fn_rev_Z 254 254 x x.
+
+(*****************************************************************************************
+ *   DEFINE SEMANTIC
+ *)
+
+Inductive expr_inv :=
+  | R_inv : expr_inv
+  | M_inv : expr_inv -> expr_inv -> expr_inv
+  | S_inv : expr_inv -> expr_inv
+  | P_inv : expr_inv -> positive -> expr_inv.
+
+Inductive formula_inv := 
+  | Eq_inv : expr_inv -> expr_inv -> formula_inv.
+
+Fixpoint expr_inv_denote v env (m : expr_inv) : Z :=
+  match m with
+  | R_inv     => term_denote env v
+  | M_inv x y => (expr_inv_denote v env x) * (expr_inv_denote v env y)
+  | S_inv x => (expr_inv_denote v env x) * (expr_inv_denote v env x)
+  | P_inv x p => Z.pow (expr_inv_denote v env x) (Z.pos p)
+  end.
+
+Definition formula_inv_denote v env (t : formula_inv) : Prop :=
+  match t with
+  | Eq_inv x y     => expr_inv_denote v env x = expr_inv_denote v env y
+  end.
+
+(*****************************************************************************************
+ *   DECIDE EQUALITY
+ *)
+
+Fixpoint compute_pow_expr_inv (t : expr_inv) : Z := match t with
+  | R_inv   => 1
+  | M_inv x y => (compute_pow_expr_inv x) + (compute_pow_expr_inv y)
+  | S_inv x => 2 * (compute_pow_expr_inv x)
+  | P_inv x p => (Z.pos p) * (compute_pow_expr_inv x)
+  end.
+
+Lemma compute_pow_expr_inv_pos : forall l, 0 <= compute_pow_expr_inv l.
+Proof. induction l ; go. Qed.
+
+Lemma compute_pow_expr_M_inv_pos : forall l l', 0 <= compute_pow_expr_inv (M_inv l l').
+Proof. intros ; simpl.
+assert(H := compute_pow_expr_inv_pos l).
+assert(H' := compute_pow_expr_inv_pos l') ; omega.
+Qed.
+
+Lemma compute_pow_expr_S_inv_pos : forall l, 0 <= compute_pow_expr_inv (S_inv l).
+Proof. intros ; simpl.
+assert(H := compute_pow_expr_inv_pos l) ; omega.
+Qed.
+
+Lemma compute_pow_expr_inv_denote: forall env v l,
+  expr_inv_denote v env l = Z.pow (term_denote env v) (compute_pow_expr_inv l).
+Proof.
+  induction l.
+  simpl ; ring.
+  assert(Hl1:= compute_pow_expr_inv_pos l1).
+  assert(Hl2:= compute_pow_expr_inv_pos l2).
+  simpl; rewrite IHl1 IHl2 -Z.pow_add_r; go.
+  assert(Hl1:= compute_pow_expr_inv_pos l).
+  simpl; rewrite IHl -Z.pow_add_r ; go.
+  f_equal ; omega.
+  assert(Hl1:= compute_pow_expr_inv_pos l).
+  assert(Hp:= Pos2Z.is_nonneg p).
+  simpl; rewrite IHl -Z.pow_mul_r; go.
+  by rewrite Z.mul_comm.
+Qed.
+
+Fixpoint decide_expr_inv_eq (l1 l2:expr_inv) :=
+  Z.eqb (compute_pow_expr_inv l1) (compute_pow_expr_inv l2).
+
+Lemma decide_expr_inv_eq_refl_impl : forall l1 l2, 
+  Z.eqb (compute_pow_expr_inv l1) (compute_pow_expr_inv l2) = true ->
+  (compute_pow_expr_inv l1) = (compute_pow_expr_inv l2).
+Proof. move=> l1 l2; rewrite Z.eqb_eq //. Qed.
+
+Lemma decide_expr_inv_eq_impl:
+  forall v env l l', 
+  decide_expr_inv_eq l l' = true ->
+  expr_inv_denote v env l = expr_inv_denote v env l'.
+Proof.
+intros; rewrite ?compute_pow_expr_inv_denote; f_equal.
+gen l'; induction l ; destruct l' ; auto => H;
+apply decide_expr_inv_eq_refl_impl in H ; by rewrite H.
+Qed.
+
+Definition decide_formula_inv (f : formula_inv) : bool := match f with
+  | Eq_inv x y => decide_expr_inv_eq x y
+  end.
+
+Lemma decide_formula_inv_impl : forall v env f, decide_formula_inv f = true -> formula_inv_denote v env f.
+Proof. move=> v env [? ?]. by apply decide_expr_inv_eq_impl. Qed.
+
+(* Weaponize our expression so we can translate functions *)
+
+
+Definition step_inv a c g : expr_inv := 
+  let c0 := (S_inv c) in if negb (Nat.eqb a 1) && negb (Nat.eqb a 3) then M_inv c0 g else c0.
+
+Lemma step_inv_step_pow_eq : forall v env a c g,
+  expr_inv_denote v env (step_inv (Z.to_nat a) c g) =  step_pow_Z a (expr_inv_denote v env c) (expr_inv_denote v env g).
+Proof.
+  intros.
+  rewrite /step_inv /step_pow_Z.
+  flatten.
+  { reflexivity. }
+  {
+  exfalso.
+  apply andb_true_iff in Eq.
+  destruct Eq as [Eq2 Eq4].
+  apply andb_false_iff in Eq0.
+  apply negb_true_iff in Eq2.
+  apply negb_true_iff in Eq4.
+  apply beq_nat_false in Eq2.
+  apply beq_nat_false in Eq4.
+  destruct Eq0 as [Eq|Eq];
+  rewrite /Zneq_bool in Eq ; flatten Eq;
+  apply Z.compare_eq_iff in Eq0 ; go.
+  }
+  {
+  exfalso.
+  apply andb_true_iff in Eq0.
+  destruct Eq0 as [Eq2 Eq4].
+  assert(a < 0 \/ 0 <= a) by omega.
+  destruct H.
+    assert(Z.to_nat a = 0%nat) by (unfold Z.to_nat ; destruct a => //).
+    rewrite H0 in Eq.
+    by compute in Eq.
+  apply andb_false_iff in Eq.
+  destruct Eq as [Eq|Eq];
+  apply negb_false_iff in Eq ; apply beq_nat_true in Eq;
+  apply (f_equal Z.of_nat) in Eq;
+  rewrite Z2Nat.id in Eq; try assumption;
+  compute in Eq;
+  subst a;
+  by compute in Eq2,Eq4.
+  }
+  { reflexivity. }
+Qed.
+
+Close Scope Z.
+
+Fixpoint pow_inv (a b : nat) (c g: expr_inv) : expr_inv := match a with
+  | 0 => c
+  | S n => let prev := pow_inv n b c g in 
+              step_inv (b - 1 - a) prev g
+  end.
+
+Open Scope Z.
+
+Lemma pow_inv_pow_fn_rev_eq : forall v env a b c g,
+  expr_inv_denote v env (pow_inv (Z.to_nat a) (Z.to_nat b) c g) =  pow_fn_rev_Z a b (expr_inv_denote v env c) (expr_inv_denote v env g).
+Proof.
+  intros.
+  destruct a; intros ; [ go | | go ].
+  remember (Z.pos p) as a.
+  assert(0 <= a) by (subst; apply Zle_0_pos).
+  clears p.
+  gen b c g.
+  gen a.
+  apply (natlike_ind (fun a => forall (b : ℤ) (c g : expr_inv),
+    expr_inv_denote v env (pow_inv (Z.to_nat a) (Z.to_nat b) c g) =
+    pow_fn_rev_Z a b (expr_inv_denote v env c) (expr_inv_denote v env g))) => //.
+  intros a Ha IHa b c g.
+  orewrite pow_fn_rev_Z_n.
+  oreplace (Z.succ a - 1) a.
+  replace ((Z.to_nat (Z.succ a))) with (S (Z.to_nat a)).
+  2: rewrite Z2Nat.inj_succ //.
+  simpl.
+  replace (Z.to_nat b - 1 - S (Z.to_nat a))%nat with (Z.to_nat (b - 1 - Z.succ a)).
+  rewrite step_inv_step_pow_eq IHa //.
+  orewrite Z2Nat.inj_sub.
+  replace ((Z.to_nat (Z.succ a))) with (S (Z.to_nat a)).
+  2: rewrite Z2Nat.inj_succ //.
+  f_equal.
+  orewrite Z2Nat.inj_sub.
+  reflexivity.
+Qed.
+
+Close Scope Z.
+
+(**************************************************************************
+ * Reflection tactics
+ *)
+
+Ltac reifyValue env t :=
+  match t with
+  | ?X =>
+    let v := lookup X env in
+    constr:(R_inv)
+  | _ => constr:(R_inv)
+  end.
+
+Ltac reifyExpr env t :=
+  lazymatch t with
+  | pow_fn_rev_Z ?a ?b ?X ?Y =>
+    let x := reifyValue env X in
+    let y := reifyValue env Y in
+    constr:(pow_inv (Z.to_nat a) (Z.to_nat b) x y)
+  | ?X * ?Y =>
+    let x := reifyValue env X in
+    let y := reifyValue env Y in
+    constr:(M_inv x y)
+  | Z.pow ?X ?Y =>
+    let x := reifyValue env X in
+    match Y with
+      | Z.pos ?p => constr:(P_inv x p)
+      | _ => constr:(P_inv x 1%positive)
+    end
+  | ?X =>
+    let x := reifyValue env X in
+    constr:(R_inv)
+  end.
+
+Ltac reifyTerm env t :=
+  lazymatch t with
+   | ?X = ?Y =>
+      let x := reifyExpr env X in
+      let y := reifyExpr env Y in
+      constr:(Eq_inv x y)
+  end.
+
+Ltac functionalize xs :=
+  let rec loop n xs' :=
+    lazymatch xs' with
+    | tt => constr:(fun _ : positive => 0%Z)
+    | (?x, tt) => constr:(fun _ : positive => x)
+    | (?x, ?xs'') =>
+      let f := loop (Pos.succ n) xs'' in
+      constr:(fun m : positive => if (m =? n)%positive then x else f m)
+    end in
+  loop (1%positive) xs.
+
+(**************************************************************************
+ * User interface tactics
+ *)
+
+Open Scope Z.
+(* 
+Eval compute in Z.pow 2 255 - 21.
+Z.pow 2 255 - 21 = 57896044618658097711785492504343953926634992332820282019728792003956564819947
+*)
+
+Theorem Inv25519_Z_correct : forall x, Inv25519_Z x = Z.pow x 57896044618658097711785492504343953926634992332820282019728792003956564819947.
+Proof.
+intros.
+  rewrite /Inv25519_Z.
+  match goal with
+  | [ |- ?X ] =>
+    let xss := constr:((x, tt)) in
+    let envv := functionalize xss in
+    let r1  := reifyTerm xss X in
+    pose xs := xss;
+    pose env := envv;
+    pose reif := r1
+    end.
+    (* in theory we would use change, but here we need to proceed slightly differently *)
+    assert (
+      formula_inv_denote (Var 1) {| vars := env |} reif ->
+      pow_fn_rev_Z 254 254 x x =
+      x ^ 57896044618658097711785492504343953926634992332820282019728792003956564819947).
+    {
+    subst env reif.
+    rewrite /formula_inv_denote pow_inv_pow_fn_rev_eq.
+    simpl. trivial.
+    }
+    apply H ; clear H.
+    apply decide_formula_inv_impl.
+    (* at this point we don't need any hypothesis, this is purely computational *)
+    subst reif ; clears.
+    compute.
+    reflexivity.
+Qed.
+
+Close Scope Z.
